src/pathfind.dfy
@@ -10,7 +10,7 @@ module Pathfind {
   // Driver method that combines the above methods to find the optimal path for an agent to reach the best visible goal in a grid environment.
   method pathfind<T>(grid: array2<T>, rectangles: array<Rectangle>, agent_position: Point, value: (Point, Point, T) -> real, traversable: T -> bool)  returns (visible: array2<bool>, path: seq<Point>)
     requires ValidPoint(agent_position, grid)
-    requires forall j :: 0 <= j < rectangles.Length ==> ValidRectangle(rectangles[j], grid)
+    requires forall j :: 0 <= j < rectangles.Length ==> RectangleInRange(rectangles[j], grid)
     ensures visible.Length0 == grid.Length0 && visible.Length1 == grid.Length1
     ensures forall i :: 0 <= i < |path| ==> ValidPoint(path[i], grid)
   {
@@ -21,37 +21,38 @@ module Pathfind {
 
   // Call once during initialization to extract rectangles from the grid then use those rectangles for all calls to pathfind function.
   method ExtractBlockingRectangles<T>(grid: array2<T>, visibility_blocking: T -> bool) returns (rectangles: array<Rectangle>)
-    ensures forall i :: 0 <= i < rectangles.Length ==> ValidRectangle(rectangles[i], grid)
+    ensures forall i :: 0 <= i < rectangles.Length ==> RectangleInRange(rectangles[i], grid)
+    ensures forall i :: 0 <= i < rectangles.Length ==> RectangleMatchesGrid(rectangles[i], grid, visibility_blocking)
   {
     var rectangles_seq := [];
-
-    var visited := new bool[grid.Length0, grid.Length1] ((i, j) => (false));
-    for x := 0 to grid.Length0 {
-      for y := 0 to grid.Length1 {
-        visited[x, y] := false;
-      }
-    }
+    var visited := new bool[grid.Length0, grid.Length1]((i, j) => false);
 
     for x := 0 to grid.Length0
-      invariant forall r :: r in rectangles_seq ==> ValidRectangle(r, grid)
+      invariant forall r :: r in rectangles_seq ==> RectangleInRange(r, grid)
+      invariant forall r :: r in rectangles_seq ==> RectangleMatchesGrid(r, grid, visibility_blocking)
     {
       for y := 0 to grid.Length1
-        invariant forall r :: r in rectangles_seq ==> ValidRectangle(r, grid)
+        invariant forall r :: r in rectangles_seq ==> RectangleInRange(r, grid)
+        invariant forall r :: r in rectangles_seq ==> RectangleMatchesGrid(r, grid, visibility_blocking)
       {
         if visibility_blocking(grid[x, y]) && !visited[x, y] {
 
-          // Determine width
           var x_size := 0;
           while x + x_size < grid.Length0 && visibility_blocking(grid[x + x_size, y]) && !visited[x + x_size, y]
             invariant x + x_size <= grid.Length0
+            invariant forall xx :: x <= xx < x + x_size ==> visibility_blocking(grid[xx, y])
           {
             x_size := x_size + 1;
           }
 
-          // Determine height
           var y_size := 1;
-          while y + y_size < grid.Length1 && forall xx {:trigger grid[xx, y + y_size]} :: x <= xx < x + x_size ==> visibility_blocking(grid[xx, y + y_size]) && !visited[xx, y + y_size]
+          while y + y_size < grid.Length1 &&
+            (forall xx {:trigger grid[xx, y + y_size]} :: x <= xx < x + x_size ==>
+            visibility_blocking(grid[xx, y + y_size]) && !visited[xx, y + y_size])
+            invariant 1 <= y_size <= grid.Length1 - y
             invariant y + y_size <= grid.Length1
+            invariant forall xx, yy :: x <= xx < x + x_size && y <= yy < y + y_size ==>
+                                         visibility_blocking(grid[xx, yy])
           {
             y_size := y_size + 1;
           }
@@ -68,6 +69,6 @@ module Pathfind {
       }
     }
 
-    rectangles := new Rectangle[|rectangles_seq|] (i requires 0<= i < |rectangles_seq| => rectangles_seq[i]);
+    rectangles := new Rectangle[|rectangles_seq|](i requires 0 <= i < |rectangles_seq| => rectangles_seq[i]);
   }
 }
